src/Validator.v
@@ -303,6 +303,15 @@ Definition storage_check_private_non_escapeb_sound :=
   check_private_non_escapeb_sound.
 Definition storage_private_non_escape_obligations :=
   private_non_escape_obligations.
+Definition storage_private_event := private_event.
+Definition storage_private_event_cell :=
+  private_event_cell.
+Definition storage_check_private_trace_cells_declaredb :=
+  check_private_trace_cells_declaredb.
+Definition storage_check_private_trace_cells_declaredb_sound :=
+  check_private_trace_cells_declaredb_sound.
+Definition storage_private_trace_cells_declared :=
+  private_trace_cells_declared.
 Definition same_instance_access_remap :=
   StorageCore.same_instance_access_remap.
 Definition same_instance_identity_remap :=
